commit

AP/System/Basic.lean
@@ -337,3 +337,12 @@ theorem simulate_eq_of_not_hasTr {f s n}
   exfalso
   apply h
   exact ⟨_, _, h₁⟩
+
+class WFTrans (sys : System S T) (t : T) : Prop where
+  h : ∃ s, sys.WF s ∧ sys.validTr s t
+
+theorem WFTrans_def {t} : sys.WFTrans t ↔ ∃ s, sys.WF s ∧ sys.validTr s t := by
+  use (·.1), (⟨·⟩)
+
+theorem wfTrans_of_tr {s s' t} [hs : sys.WF s]
+(h : sys.tr s t = some s') : sys.WFTrans t := by use s, hs, s'
