AP/System/Symmetry.lean
@@ -5,25 +5,155 @@ namespace System
 universe u
 variable {S T : Type u} {sys : System S T}
 
+@[ext]
 structure Symmetry (sys : System S T) : Type u where
   fs : S → S
+  fs' : S → S
   ft : T → T
+  ft' : T → T
 
 namespace Symmetry
 
 variable {sym : sys.Symmetry}
 
 class WF (sym : sys.Symmetry) : Prop where
-  tr_eq : ∀ {s t} [sys.WF s], sys.tr (sym.fs s) (sym.ft t) = (sys.tr s t).map sym.fs
+  h_fs : Function.BijectiveOn sys.WF sys.WF sym.fs sym.fs'
+  h_ft : Function.BijectiveOn sys.WFTrans sys.WFTrans sym.ft sym.ft'
+  tr_eq : ∀ {s t} [sys.WF s], sys.tr s t = (sys.tr (sym.fs s) (sym.ft t)).map sym.fs'
+  tr_eq' : ∀ {s t} [sys.WF s], sys.tr s t = (sys.tr (sym.fs' s) (sym.ft' t)).map sym.fs
 
-theorem wf_def : sym.WF ↔ ∀ {s t} [sys.WF s],
-sys.tr (sym.fs s) (sym.ft t) = (sys.tr s t).map sym.fs := ⟨(·.1), (⟨·⟩)⟩
+instance : Inhabited (Symmetry sys) := ⟨id, id, id, id⟩
 
-def tr_eq {s t} [hs : sys.WF s] [h : sym.WF] :
-sys.tr (sym.fs s) (sym.ft t) = (sys.tr s t).map sym.fs := h.tr_eq
+theorem default_eq : (default : Symmetry sys) = ⟨id, id, id, id⟩ := rfl
 
-instance : Inhabited (Symmetry sys) := ⟨id, id⟩
+@[simp]
+instance : (default : Symmetry sys).WF := by
+  rw [default_eq]; constructor <;> simp
 
-theorem default_eq : (default : Symmetry sys) = ⟨id, id⟩ := rfl
+instance {s} [H : sym.WF] [hs : sys.WF s] : sys.WF (sym.fs s) :=
+  H.h_fs.cnd_right hs
 
-@[simp] instance : (default : Symmetry sys).WF := by simp [wf_def, default_eq]
+instance {s} [H : sym.WF] [hs : sys.WF s] : sys.WF (sym.fs' s) :=
+  H.h_fs.cnd_left hs
+
+instance {t} [H : sym.WF] [ht : sys.WFTrans t] : sys.WFTrans (sym.ft t) :=
+  H.h_ft.cnd_right ht
+
+instance {t} [H : sym.WF] [ht : sys.WFTrans t] : sys.WFTrans (sym.ft' t) :=
+  H.h_ft.cnd_left ht
+
+@[simp]
+theorem fs'_fs {s} [H : sym.WF] [hs : sys.WF s] : sym.fs' (sym.fs s) = s :=
+  H.h_fs.cancel_left hs
+
+@[simp]
+theorem fs_fs' {s} [H : sym.WF] [hs : sys.WF s] : sym.fs (sym.fs' s) = s :=
+  H.h_fs.cancel_right hs
+
+@[simp]
+theorem ft'_ft {t} [H : sym.WF] [ht : sys.WFTrans t] : sym.ft' (sym.ft t) = t :=
+  H.h_ft.cancel_left ht
+
+@[simp]
+theorem ft_ft' {t} [H : sym.WF] [ht : sys.WFTrans t] : sym.ft (sym.ft' t) = t :=
+  H.h_ft.cancel_right ht
+
+def tr_fs {s t} [H : sym.WF] [hs : sys.WF s] :
+sys.tr (sym.fs s) t = (sys.tr s (sym.ft' t)).map sym.fs := by
+  nth_rw 1 [H.tr_eq']; ext s'; simp
+
+def tr_fs' {s t} [H : sym.WF] [hs : sys.WF s] :
+sys.tr (sym.fs' s) t = (sys.tr s (sym.ft t)).map sym.fs' := by
+  nth_rw 1 [H.tr_eq]; ext s'; simp
+
+def tr_ft {s t} [H : sym.WF] [hs : sys.WF s] :
+sys.tr s (sym.ft t) = (sys.tr (sym.fs' s) t).map sym.fs := by
+  nth_rw 2 [H.tr_eq]; ext s'; simp; constructor
+  · intro h; use s'; have hs' := wf_of_tr h; simpa
+  · rintro ⟨s₁, h₁, h₂⟩; have hs₁ := wf_of_tr h₁; simp at h₂; simpa [←h₂]
+
+def tr_ft' {s t} [H : sym.WF] [hs : sys.WF s] :
+sys.tr s (sym.ft' t) = (sys.tr (sym.fs s) t).map sym.fs' := by
+  nth_rw 2 [H.tr_eq']; ext s'; simp; constructor
+  · intro h; use s', h; have h₁ := wf_of_tr h; simp
+  · rintro ⟨s₁, h₁, h₂⟩; have h₃ := wf_of_tr h₁; simp at h₂; simpa [←h₂]
+
+theorem validTr_fs_of {s t} [H : sym.WF] [hs : sys.WF s]
+(h : sys.validTr s (sym.ft' t)) : sys.validTr (sym.fs s) t := by
+  obtain ⟨s', h⟩ := h; simp [tr_ft'] at h; obtain ⟨s', h, rfl⟩ := h; use s'
+
+theorem validTr_fs'_of {s t} [H : sym.WF] [hs : sys.WF s]
+(h : sys.validTr s (sym.ft t)) : sys.validTr (sym.fs' s) t := by
+  obtain ⟨s', h⟩ := h; simp [tr_ft] at h; obtain ⟨s', h, rfl⟩ := h; use s'
+
+theorem validTr_ft_of {s t} [H : sym.WF] [hs : sys.WF s]
+(h : sys.validTr (sym.fs' s) t) : sys.validTr s (sym.ft t) := by
+  obtain ⟨s', h⟩ := h; simp [tr_fs'] at h; obtain ⟨s', h, rfl⟩ := h; use s'
+
+theorem validTr_ft'_of {s t} [H : sym.WF] [hs : sys.WF s]
+(h : sys.validTr (sym.fs s) t) : sys.validTr s (sym.ft' t) := by
+  obtain ⟨s', h⟩ := h; simp [tr_fs] at h; obtain ⟨s', h, rfl⟩ := h; use s'
+
+theorem validTr_fs {s t} [H : sym.WF] [hs : sys.WF s] :
+sys.validTr (sym.fs s) t ↔ sys.validTr s (sym.ft' t) :=
+  ⟨validTr_ft'_of, validTr_fs_of⟩
+
+theorem validTr_fs' {s t} [H : sym.WF] [hs : sys.WF s] :
+sys.validTr (sym.fs' s) t ↔ sys.validTr s (sym.ft t) :=
+  ⟨validTr_ft_of, validTr_fs'_of⟩
+
+theorem validTr_ft {s t} [H : sym.WF] [hs : sys.WF s] :
+sys.validTr s (sym.ft t) ↔ sys.validTr (sym.fs' s) t :=
+  ⟨validTr_fs'_of, validTr_ft_of⟩
+
+theorem validTr_ft' {s t} [H : sym.WF] [hs : sys.WF s] :
+sys.validTr s (sym.ft' t) ↔ sys.validTr (sym.fs s) t :=
+  ⟨validTr_fs_of, validTr_ft'_of⟩
+
+@[simp]
+theorem hasTr_fs {s} [H : sym.WF] [hs : sys.WF s] :
+sys.hasTr (sym.fs s) ↔ sys.hasTr s := by
+  constructor <;> rintro ⟨t, h⟩
+  · use sym.ft' t; simpa [validTr_ft']
+  · use sym.ft t; simpa [validTr_ft]
+
+@[simp]
+theorem hasTr_fs' {s} [H : sym.WF] [hs : sys.WF s] :
+sys.hasTr (sym.fs' s) ↔ sys.hasTr s := by
+  constructor <;> rintro ⟨t, h⟩
+  · use sym.ft t; simpa [validTr_ft]
+  · use sym.ft' t; simpa [validTr_ft']
+
+example {s t} [H : sym.WF] [hs : sys.WF s] :
+sys.validTr (sym.fs s) t ↔ sys.validTr s (sym.ft' t) := by
+  symm; constructor
+  · exact fun a ↦ validTr_fs_of a
+  · exact fun a ↦ validTr_ft'_of a
+
+@[simp]
+def simFn (sym : Symmetry sys) (f : S → T) (s : S) : T :=
+  sym.ft # f # sym.fs' s
+
+instance {f} [H : sym.WF] [hf : sys.SimFn f] : sys.SimFn (sym.simFn f) := by
+  rw [sys.simFn_def]; intro s hs h; simp; apply hf.1 at h; apply validTr_ft_of
+  have h₁ : sys.hasTr (sym.fs' s); simp; exact ⟨_, h⟩; exact hf.1 h₁
+
+def inv (sym : Symmetry sys) : Symmetry sys where
+  fs := sym.fs'
+  fs' := sym.fs
+  ft' := sym.ft
+  ft := sym.ft'
+
+@[simp]
+theorem inv_inv : sym.inv.inv = sym := by ext <;> rfl
+
+instance [H : sym.WF] : sym.inv.WF where
+  h_fs := H.h_fs.symm
+  h_ft := H.h_ft.symm
+  tr_eq := WF.tr_eq'
+  tr_eq' := WF.tr_eq
+
+@[simp]
+theorem wf_inv_iff : sym.inv.WF ↔ sym.WF := by
+  symm; constructor <;> intro h; infer_instance
+  rw [←sym.inv_inv]; infer_instance
